remove handle_pts_to, thread log from preconds (assume thread locks)

steel/Zeta.Steel.SafeMain.fst
@@ -6,32 +6,32 @@ module R = Steel.ST.Reference
 open Steel.ST.GenElim
 
 [@@__reduce__]
-let state_ptr_has_core_inv_false
+let state_ptr_inv_null
   (p: perm)
 : Tot vprop
 = pure (p == full_perm)
 
 [@@__reduce__]
-let state_ptr_has_core_inv_true
+let state_ptr_inv_not_null
   (state: R.ref M.top_level_state)
 : Tot vprop
-= exists_ (fun ps -> exists_ (fun ts -> R.pts_to state ps ts `star` M.core_inv ts))
+= exists_ (fun pt -> exists_ (fun t -> R.pts_to state pt t `star` M.core_inv t))
 
-let state_ptr_has_core_inv
-  (p: perm)
+let state_ptr_inv_if
   (state: R.ref M.top_level_state)
+  (p: perm)
 : Tot vprop
 = if R.is_null state
-  then state_ptr_has_core_inv_false p
-  else state_ptr_has_core_inv_true state
+  then state_ptr_inv_null p
+  else state_ptr_inv_not_null state
 
 [@@__reduce__]
 let state_ptr_inv0
   (state_ptr: R.ref (R.ref M.top_level_state))
 : Tot vprop
-= exists_ (fun (p: perm) -> exists_ (fun (state: R.ref M.top_level_state) ->
-    R.pts_to state_ptr p state `star`
-    state_ptr_has_core_inv p state
+= exists_ (fun p -> exists_ (fun state ->
+    R.pts_to state_ptr (half_perm p) state `star`
+    state_ptr_inv_if state p
   ))
 
 let state_ptr_inv
@@ -39,25 +39,48 @@ let state_ptr_inv
 : Tot vprop
 = state_ptr_inv0 state_ptr
 
+let state_ptr_lock_prop
+  (state: R.ref M.top_level_state)
+  (p: perm)
+: Tot prop
+= R.is_null state == true ==> p == full_perm
+
+[@@__reduce__]
+let state_ptr_lock0
+  (state_ptr: R.ref (R.ref M.top_level_state))
+: Tot vprop
+= exists_ (fun p -> exists_ (fun state ->
+    R.pts_to state_ptr (half_perm p) state `star`
+    pure (state_ptr_lock_prop state p)
+  ))
+
+let state_ptr_lock
+  (state_ptr: R.ref (R.ref M.top_level_state))
+: Tot vprop
+= state_ptr_lock0 state_ptr
+
 noeq
 type handle_t = {
   state_ptr: R.ref (R.ref M.top_level_state);
-  lock: Lock.lock (state_ptr_inv state_ptr);
+  _inv: inv (state_ptr_inv state_ptr);
+  _lock: Lock.lock (state_ptr_lock state_ptr);
 }
 
 let create_handle () : STT handle_t emp (fun _ -> emp) =
   let state_ptr : R.ref (R.ref M.top_level_state) = R.alloc R.null in
-  noop ();
-  rewrite
-    (state_ptr_has_core_inv_false full_perm)
-    (state_ptr_has_core_inv full_perm R.null);
-  rewrite
-    (state_ptr_inv0 state_ptr)
-    (state_ptr_inv state_ptr);
-  let lock = Lock.new_lock (state_ptr_inv state_ptr) in
+  R.share state_ptr;
+  (* invariant *)
+  rewrite (state_ptr_inv_null full_perm) (state_ptr_inv_if R.null full_perm);
+  rewrite (state_ptr_inv0 state_ptr) (state_ptr_inv state_ptr);
+  let _inv = new_invariant (state_ptr_inv state_ptr) in
+  (* lock *)
+  rewrite (state_ptr_lock0 state_ptr) (state_ptr_lock state_ptr);
+  let _lock = Lock.new_lock (state_ptr_lock state_ptr) in
+  (* summary *)
   return ({
     state_ptr = state_ptr;
-    lock = lock;
+    _inv = _inv;
+    _lock = _lock;
   })
 
 (* FIXME: this makes F* crash with
@@ -128,95 +151,401 @@ let share
   noop ();
   rewrite (handle_pts_to0 ts) (handle_pts_to ts)
 
-#push-options "--z3rlimit 16"
+let with_invariant_g (#a:Type)
+                     (#fp:vprop)
+                     (#fp':a -> vprop)
+                     (#opened_invariants:inames)
+                     (#p:vprop)
+                     (i:inv p{not (mem_inv opened_invariants i)})
+                     (f:unit -> STGhostT a (add_inv opened_invariants i)
+                                         (p `star` fp)
+                                         (fun x -> p `star` fp' x))
+  : STGhostT a opened_invariants fp fp'
+= with_invariant_g i f
+
+let gen_handle_pts_to_not_null
+  (#opened: _)
+  (#p: _)
+  (#state: _)
+  ()
+: STGhost (Ghost.erased M.top_level_state) opened
+    (R.pts_to handle.state_ptr p state)
+    (fun ts -> exists_ (fun p' -> R.pts_to handle.state_ptr (half_perm p') state) `star` handle_pts_to ts)
+    ((not (mem_inv opened handle._inv)) /\
+      (not (R.is_null state))
+    )
+    (fun _ -> True)
+= noop (); // for pure
+  with_invariant_g
+    #(Ghost.erased M.top_level_state)
+    #(R.pts_to handle.state_ptr p state `star` pure (R.is_null state == false))
+    #(fun ts -> (exists_ (fun p' -> R.pts_to handle.state_ptr (half_perm p') state) `star` handle_pts_to ts))
+    #opened
+    #(state_ptr_inv handle.state_ptr)
+    handle._inv
+    (fun _ ->
+      rewrite
+        (state_ptr_inv handle.state_ptr)
+        (state_ptr_inv0 handle.state_ptr);
+      let _ = gen_elim () in
+      R.gather p handle.state_ptr;
+      vpattern_rewrite (R.pts_to handle.state_ptr _) state;
+      rewrite
+        (state_ptr_inv_if _ _)
+        (state_ptr_inv_not_null state);
+      let _ = gen_elim () in
+      let ts = vpattern_replace_erased (fun ts -> R.pts_to state _ ts `star` M.core_inv ts) in
+      R.share state;
+      M.core_inv_share ts;
+      R.share handle.state_ptr;
+      (* handle_pts_to *)
+      rewrite (handle_pts_to0 ts) (handle_pts_to ts);
+      let p' = vpattern_replace (fun p' -> R.pts_to handle.state_ptr p' _) in
+      R.share handle.state_ptr;
+      (* invariant *)
+      rewrite
+        (state_ptr_inv_not_null state)
+        (state_ptr_inv_if state p');
+      rewrite
+        (state_ptr_inv0 handle.state_ptr)
+        (state_ptr_inv handle.state_ptr);
+      (* postcond *)
+      noop ();
+      ts
+    )
+
+assume
+val atomic_read_ref
+  (#t: Type)
+  (#opened:_)
+  (#p:perm)
+  (#v:Ghost.erased t)
+  (r:R.ref t)
+  : STAtomic t opened
+      (R.pts_to r p v)
+      (fun x -> R.pts_to r p v)
+      (requires True)
+      (ensures fun x -> x == Ghost.reveal v)
+
+assume
+val atomic_write_ref
+  (#t: Type)
+  (#opened:_)
+  (#v:Ghost.erased t)
+  (r:R.ref t)
+  (x:t)
+  : STAtomicT unit opened
+      (R.pts_to r full_perm v)
+      (fun _ -> R.pts_to r full_perm x)
+
+let handle_is_null_post (b: bool) : vprop =
+  if b
+  then emp
+  else exists_ handle_pts_to
+
+inline_for_extraction
+let with_invariant (#a:Type)
+                   (#fp:vprop)
+                   (#fp':a -> vprop)
+                   (#opened_invariants:inames)
+                   (#p:vprop)
+                   (i:inv p{not (mem_inv opened_invariants i)})
+                   (f:unit -> STAtomicT a (add_inv opened_invariants i)
+                                          (p `star` fp)
+                                          (fun x -> p `star` fp' x))
+  : STAtomicT a opened_invariants fp fp'
+= with_invariant i f
+
+let handle_is_null
+  (#opened: _)
+  ()
+: STAtomic bool opened
+    emp
+    (fun b -> handle_is_null_post b)
+    (not (mem_inv opened handle._inv))
+    (fun _ -> True)
+= noop (); // for pure
+  with_invariant
+    #bool
+    #emp
+    #(fun b -> handle_is_null_post b)
+    #_
+    #(state_ptr_inv handle.state_ptr)
+    handle._inv
+    (fun _ ->
+      rewrite
+        (state_ptr_inv handle.state_ptr)
+        (state_ptr_inv0 handle.state_ptr);
+      let _ = gen_elim () in
+      let state = atomic_read_ref handle.state_ptr in
+      if R.is_null state
+      then begin
+        noop ();
+        rewrite
+          (state_ptr_inv0 handle.state_ptr)
+          (state_ptr_inv handle.state_ptr);
+        rewrite
+          emp
+          (handle_is_null_post true);
+        return true
+      end else begin
+        let p = vpattern_replace (fun p -> R.pts_to handle.state_ptr (half_perm p) _ `star` state_ptr_inv_if _ p) in
+        let state = vpattern_replace_erased (fun state -> R.pts_to handle.state_ptr _ state `star` state_ptr_inv_if state _) in
+        rewrite
+          (state_ptr_inv_if _ _)
+          (state_ptr_inv_not_null state);
+        let _ = gen_elim () in
+        R.share handle.state_ptr;
+        R.share state;
+        M.core_inv_share _;
+        (* invariant *)
+        rewrite
+          (state_ptr_inv_not_null state)
+          (state_ptr_inv_if state (half_perm p));
+        rewrite
+          (state_ptr_inv0 handle.state_ptr)
+          (state_ptr_inv handle.state_ptr);
+        (* handle_pts_to *)
+        let ts = vpattern_replace_erased (fun ts -> R.pts_to state _ ts `star` M.core_inv ts) in
+        rewrite
+          (handle_pts_to0 ts)
+          (handle_pts_to ts);
+        rewrite 
+          (exists_ handle_pts_to)
+          (handle_is_null_post false);
+        return false
+      end
+    )
+
+#push-options "--z3rlimit 32"
 #restart-solver
 
 let init ()
-= Lock.acquire handle.lock;
-  rewrite (state_ptr_inv handle.state_ptr) (state_ptr_inv0 handle.state_ptr);
+= Lock.acquire handle._lock;
+  rewrite (state_ptr_lock handle.state_ptr) (state_ptr_lock0 handle.state_ptr);
   let _ = gen_elim () in
   let state = R.read handle.state_ptr in
-  vpattern_rewrite (state_ptr_has_core_inv _) state;
-  let p = vpattern_replace (fun p -> state_ptr_has_core_inv p _) in
   if R.is_null state
   then begin
-    rewrite (state_ptr_has_core_inv _ _) (state_ptr_has_core_inv_false p);
-    let _ = gen_elim () in
-    let state = M.init () in
+    let state' = M.init () in
     let ts = elim_exists () in
+    R.pts_to_not_null state';
+    rewrite (R.pts_to handle.state_ptr _ _) (R.pts_to handle.state_ptr (half_perm full_perm) state);
     M.core_inv_share ts;
-    R.pts_to_not_null state;
-    vpattern_rewrite (fun p -> R.pts_to handle.state_ptr p _) full_perm;
-    R.write handle.state_ptr state;
+    R.share state';
+    with_invariant
+      #unit
+      #(R.pts_to handle.state_ptr (half_perm full_perm) state `star` R.pts_to state' (half_perm full_perm) ts `star` M.core_inv ts)
+      #(fun _ -> R.pts_to handle.state_ptr (half_perm full_perm) state')
+      #_
+      #(state_ptr_inv handle.state_ptr)
+      (handle._inv)
+      (fun _ ->
+        rewrite (state_ptr_inv handle.state_ptr) (state_ptr_inv0 handle.state_ptr);
+        let _ = gen_elim () in
+        R.gather (half_perm full_perm) handle.state_ptr;
+        let p = vpattern_replace (state_ptr_inv_if _) in
+        rewrite
+          (state_ptr_inv_if _ _)
+          (state_ptr_inv_null p);
+        let _ = gen_elim () in
+        vpattern_rewrite (fun p -> R.pts_to handle.state_ptr p _) full_perm;
+        atomic_write_ref handle.state_ptr state';
+        R.share handle.state_ptr;
+        noop ();
+        rewrite
+          (state_ptr_inv_not_null state')
+          (state_ptr_inv_if state' full_perm);
+        rewrite
+          (state_ptr_inv0 handle.state_ptr)
+          (state_ptr_inv handle.state_ptr)
+      );
     R.share handle.state_ptr;
-    R.share state;
-    rewrite (state_ptr_has_core_inv_true state) (state_ptr_has_core_inv (half_perm full_perm) state);
-    rewrite (state_ptr_inv0 handle.state_ptr) (state_ptr_inv handle.state_ptr);
-    Lock.release handle.lock;
+    rewrite (state_ptr_lock0 handle.state_ptr) (state_ptr_lock handle.state_ptr);
+    Lock.release handle._lock;
     rewrite (handle_pts_to0 ts) (handle_pts_to ts);
     rewrite (init_post_true ts) (init_post true ts);
     return true
   end else begin
-    rewrite (state_ptr_has_core_inv _ _) (state_ptr_has_core_inv_true state);
+    let ts = gen_handle_pts_to_not_null () in
     let _ = gen_elim () in
-    let ts = vpattern_replace_erased (fun ts -> R.pts_to state _ ts `star` M.core_inv ts) in
-    R.share state;
-    M.core_inv_share ts;
-    rewrite (R.pts_to handle.state_ptr _ _) (R.pts_to handle.state_ptr p state);
-    R.share handle.state_ptr;
-    rewrite (state_ptr_has_core_inv_true state) (state_ptr_has_core_inv (half_perm p) state);
-    rewrite (state_ptr_inv0 handle.state_ptr) (state_ptr_inv handle.state_ptr);
-    Lock.release handle.lock;
-    rewrite (handle_pts_to0 ts) (handle_pts_to ts);
+    rewrite (state_ptr_lock0 handle.state_ptr) (state_ptr_lock handle.state_ptr);
+    Lock.release handle._lock;
     rewrite emp (init_post false ts);
     return false
   end
 
 #pop-options
 
-let verify_log
-               (#t:Ghost.erased M.top_level_state)
-               (tid:_)
-               (#entries:Ghost.erased AEH.log)
+assume val acquire_thread_lock
+  (t: Ghost.erased M.top_level_state)
+  (tid: AT.tid)
+: STT (Ghost.erased AEH.log)
+    (handle_pts_to t)
+    (fun entries -> handle_pts_to t `star` M.log_of_tid t tid entries)
+
+assume val release_thread_lock
+  (t: Ghost.erased (M.top_level_state))
+  (tid: AT.tid)
+  (entries: Ghost.erased AEH.log)
+: STT unit
+    (handle_pts_to t `star` M.log_of_tid t tid entries)
+    (fun _ -> handle_pts_to t)
+
+#push-options "--z3rlimit 32 --query_stats --ifuel 6"
+#restart-solver
+
+let m_verify_post_failure_eq
+  (#opened: _)
+  (t:M.top_level_state)
+  (tid:AT.tid)
+  (entries:Ghost.erased AEH.log)
+  (log_perm:perm)
+  (log_bytes:Ghost.erased AT.bytes)
+  (len: U32.t)
+  (input:U.larray U8.t len)
+  (out_len: U32.t)
+  (out_bytes:Ghost.erased AT.bytes)
+  (output:U.larray U8.t out_len)
+  (res: (option (v:V.verify_result { V.verify_result_complete len v })))
+: STGhost unit opened
+  (
+    M.verify_post t tid entries log_perm log_bytes len input out_len out_bytes output res
+  )
+  (fun _ ->
+    M.core_inv t `star`
+    A.pts_to input log_perm log_bytes `star` (
+       exists_ (fun s -> A.pts_to output full_perm s) `star`
+       exists_ (fun entries' -> M.log_of_tid t tid entries'))
+  )
+  (match res with
+  | Some (V.Verify_success _ _) -> False
+  | _ -> True
+  )
+  (fun _ -> True)
+= rewrite
+    (M.verify_post t tid entries log_perm log_bytes len input out_len out_bytes output res)
+    (M.core_inv t `star`
+    A.pts_to input log_perm log_bytes `star` (
+       exists_ (fun s -> A.pts_to output full_perm s) `star`
+       exists_ (fun entries' -> M.log_of_tid t tid entries')))
+
+let verify_log_some
+               (t: Ghost.erased M.top_level_state)
+               (tid:U16.t)
                (#log_perm:perm)
                (#log_bytes:Ghost.erased AT.bytes)
-               (len: U32.t { len <> 0ul })
-               (input:U.larray U8.t len)
+               (len: U32.t)
+               (input: EXT.extern_ptr U8.t)
                (out_len: U32.t)
                (#out_bytes:Ghost.erased AT.bytes)
-               (output:U.larray U8.t out_len)
-  : STT (option (v:V.verify_result { V.verify_result_complete len v }))
-    (handle_pts_to t `star`
-     A.pts_to input log_perm log_bytes `star`
-     A.pts_to output full_perm out_bytes `star`
-     M.log_of_tid t tid entries)
-    (fun res ->
-       handle_pts_to t `star`
-       M.verify_post t tid entries log_perm log_bytes len input out_len out_bytes output res)
-= rewrite (handle_pts_to t) (handle_pts_to0 t);
-  let _ = gen_elim () in
-  let state = R.read handle.state_ptr in
-  vpattern_rewrite (R.pts_to handle.state_ptr _) state;
-  vpattern_rewrite (fun (state: R.ref M.top_level_state) -> R.pts_to state _ t) state;
-  M.core_inv_share t;
-  let res = M.verify_log state tid len input out_len output in
-  rewrite (handle_pts_to0 t) (handle_pts_to t);
-  return res
-
-let max_certified_epoch
-                        (#t:Ghost.erased M.top_level_state)
-                        (_: unit)
-  : STT AEH.max_certified_epoch_result
-        (handle_pts_to t)
-        (fun res ->
-           handle_pts_to t `star`
-           M.read_max_post t res)
-=
+               (output: EXT.extern_ptr U8.t)
+  : ST (verify_result len)
+    (handle_pts_to t `star` verify_pre log_perm log_bytes input out_bytes output)
+    (fun res -> verify_post tid log_perm log_bytes len input out_len out_bytes output res)
+    (check_verify_input tid len input out_len output)
+    (fun _ -> True)
+= let entries = acquire_thread_lock t tid in
   rewrite (handle_pts_to t) (handle_pts_to0 t);
   let _ = gen_elim () in
   let state = R.read handle.state_ptr in
   vpattern_rewrite (R.pts_to handle.state_ptr _) state;
   vpattern_rewrite (fun (state: R.ref M.top_level_state) -> R.pts_to state _ t) state;
-  let res = M.max_certified_epoch state in
-  rewrite (handle_pts_to0 t) (handle_pts_to t);
-  return res
+  let input' = EXT.take input len in
+  let output' = EXT.take output out_len in
+  vpattern_rewrite (fun a -> A.pts_to a log_perm log_bytes) input';
+  vpattern_rewrite (fun a -> A.pts_to a full_perm out_bytes) output';
+  let v = M.verify_log state tid len input' out_len output' in
+  let res = Some v in
+  match v returns STT (verify_result len) (R.pts_to handle.state_ptr _ _ `star` R.pts_to state _ _ `star`  M.verify_post t tid entries log_perm log_bytes len input' out_len out_bytes output' v) (fun res -> verify_post tid log_perm log_bytes len input out_len out_bytes output res) with
+  | Some (V.Verify_success read wrote) ->
+    rewrite
+      (M.verify_post t tid entries log_perm log_bytes len input' out_len out_bytes output' _)
+      (M.core_inv t `star`
+        A.pts_to (EXT.gtake input) log_perm log_bytes `star`
+        exists_ (M.verify_post_success_pred t tid entries log_bytes out_len out_bytes output' read wrote)
+      );
+    let _ = gen_elim () in
+    rewrite (handle_pts_to0 t) (handle_pts_to t);
+    let entries' = vpattern_erased (fun entries' -> M.log_of_tid t tid (_ `Seq.append` entries')) in
+    let out_bytes' = vpattern_replace_erased (A.pts_to output' _) in
+    release_thread_lock t tid _;
+    vpattern_rewrite #_ #_ #output' (fun output -> A.pts_to output _ _) (EXT.gtake output);
+    assert_ (verify_post_some_m_success_body tid log_perm log_bytes len input out_len out_bytes output v () t entries read wrote entries' out_bytes');
+    rewrite
+      (verify_post_some_m_success tid log_perm log_bytes len input out_len out_bytes output v () t entries read wrote)
+      (verify_post_some_m tid log_perm log_bytes len input out_len out_bytes output v () t entries);
+    rewrite
+      (verify_post_some tid log_perm log_bytes len input out_len out_bytes output v ())
+      (verify_post tid log_perm log_bytes len input out_len out_bytes output res);
+    return res
+  | v ->
+    m_verify_post_failure_eq t tid entries log_perm log_bytes len input' out_len out_bytes output' v;
+    let _ = gen_elim () in
+    rewrite (handle_pts_to0 t) (handle_pts_to t);
+    release_thread_lock t tid _;
+    vpattern_rewrite #_ #_ #output' (fun output -> A.pts_to output _ _) (EXT.gtake output);
+    rewrite
+      (verify_post_some_m_failure output)
+      (verify_post_some_m tid log_perm log_bytes len input out_len out_bytes output v () t entries);
+    vpattern_rewrite #_ #_ #input' (fun input -> A.pts_to input _ _) (EXT.gtake input);
+    rewrite
+      (verify_post_some tid log_perm log_bytes len input out_len out_bytes output v ())
+      (verify_post tid log_perm log_bytes len input out_len out_bytes output res);
+    return res
+
+let verify_log
+  tid #log_perm #log_bytes len input out_len #out_bytes output
+=
+  if not (check_verify_input tid len input out_len output) returns STT (verify_result len)
+    (verify_pre log_perm log_bytes input out_bytes output)
+    (fun res -> verify_post tid log_perm log_bytes len input out_len out_bytes output res)
+  then begin
+    noop ();
+    rewrite (verify_pre log_perm log_bytes input out_bytes output)
+      (verify_post tid log_perm log_bytes len input out_len out_bytes output None);
+    return None
+  end else
+  let is_null = handle_is_null () in
+  if is_null
+  then begin
+    noop ();
+    rewrite (handle_is_null_post _) emp;
+    rewrite (verify_pre log_perm log_bytes input out_bytes output)
+      (verify_post tid log_perm log_bytes len input out_len out_bytes output None);
+    return None
+  end else 
+  begin
+    noop ();
+    rewrite (handle_is_null_post _) (exists_ handle_pts_to);
+    let ts = elim_exists () in
+    verify_log_some ts tid len input out_len output
+  end
+
+let max_certified_epoch
+  ()
+=
+  let is_null = handle_is_null () in
+  if is_null
+  then begin
+    noop ();
+    rewrite (handle_is_null_post _) (max_certified_epoch_post None);
+    return None
+  end else 
+  begin
+    noop ();
+    rewrite (handle_is_null_post _) (exists_ handle_pts_to);
+    let t = elim_exists () in
+    rewrite (handle_pts_to t) (handle_pts_to0 t);
+    let _ = gen_elim () in
+    let state = R.read handle.state_ptr in
+    vpattern_rewrite (R.pts_to handle.state_ptr _) state;
+    vpattern_rewrite (fun (state: R.ref M.top_level_state) -> R.pts_to state _ t) state;
+    let r = M.max_certified_epoch state in
+    rewrite (handle_pts_to0 t) (handle_pts_to t);
+    let res = Some r in
+    rewrite (max_certified_epoch_post_some r) (max_certified_epoch_post res);
+    return res
+  end
+
+#pop-options
