steel/Zeta.Steel.SafeMain.fsti
@@ -1,6 +1,16 @@
 module Zeta.Steel.SafeMain
 
 module M = Zeta.Steel.Main
+module AEH = Zeta.Steel.AggregateEpochHashes
+module U32 = FStar.UInt32
+module U8 = FStar.UInt8
+module U = Zeta.Steel.Util
+module V = Zeta.Steel.Verifier
+module A = Steel.ST.Array
+module AT = Zeta.Steel.ApplicationTypes
+module EXT = Zeta.Steel.ExternalPtr
+module U16 = FStar.UInt16
+
 open Steel.ST.Util
 
 val handle_pts_to
@@ -59,39 +69,179 @@ val init (_: unit) : STT bool
       init_post b ts
   ))
 
-module AEH = Zeta.Steel.AggregateEpochHashes
-module U32 = FStar.UInt32
-module U8 = FStar.UInt8
-module U = Zeta.Steel.Util
-module V = Zeta.Steel.Verifier
-module A = Steel.ST.Array
-module AT = Zeta.Steel.ApplicationTypes
+let verify_result (len: U32.t) = option (option (v:V.verify_result { V.verify_result_complete len v }))
+
+[@__reduce__]
+let verify_pre
+    (log_perm:perm)
+    (log_bytes: AT.bytes)
+    (input: EXT.extern_ptr U8.t)
+    (out_bytes: AT.bytes)
+    (output: EXT.extern_ptr U8.t)
+: Tot vprop
+=
+     A.pts_to (EXT.gtake input) log_perm log_bytes `star`
+     A.pts_to (EXT.gtake output) full_perm out_bytes
+
+inline_for_extraction
+let check_verify_input
+  (tid: U16.t)
+  (len: U32.t) // { len <> 0ul })
+  (input: EXT.extern_ptr U8.t) // U.larray U8.t len)
+  (out_len: U32.t)
+  (output: EXT.extern_ptr U8.t) // U.larray U8.t out_len)
+: Tot bool
+= FStar.Int.Cast.uint16_to_uint32 tid `U32.lt` AT.n_threads &&
+  len <> 0ul &&
+  EXT.valid input len &&
+  EXT.valid output out_len
+
+[@@__reduce__]
+let verify_post_some_m_success_body
+  (tid:U16.t)
+  (log_perm:perm)
+  (log_bytes: AT.bytes)
+  (len: U32.t) // { len <> 0ul })
+  (input: EXT.extern_ptr U8.t) // U.larray U8.t len)
+  (out_len: U32.t)
+  (out_bytes: AT.bytes)
+  (output: EXT.extern_ptr U8.t) // U.larray U8.t out_len)
+  (v: option (v:V.verify_result { V.verify_result_complete len v }))
+  (sq: squash (check_verify_input tid len input out_len output))
+  (t: M.top_level_state)
+  (entries: _)
+  (read:U32.t)
+  (wrote:U32.t)
+  (entries' : _)
+  (out_bytes' : _)
+: Tot vprop
+=        A.pts_to (EXT.gtake output) full_perm out_bytes'
+           `star`
+         pure (M.verify_post_success_pure_inv
+            tid
+            entries
+            log_bytes
+            out_bytes
+            read
+            wrote
+            entries'
+            out_bytes')
+
+[@@__reduce__]
+let verify_post_some_m_success
+  (tid:U16.t)
+  (log_perm:perm)
+  (log_bytes: AT.bytes)
+  (len: U32.t) // { len <> 0ul })
+  (input: EXT.extern_ptr U8.t) // U.larray U8.t len)
+  (out_len: U32.t)
+  (out_bytes: AT.bytes)
+  (output: EXT.extern_ptr U8.t) // U.larray U8.t out_len)
+  (v: option (v:V.verify_result { V.verify_result_complete len v }))
+  (sq: squash (check_verify_input tid len input out_len output))
+  (t: M.top_level_state)
+  (entries: _)
+  (read:U32.t)
+  (wrote:U32.t)
+: Tot vprop
+=
+       exists_ (fun entries' -> exists_ (fun out_bytes' ->
+         verify_post_some_m_success_body tid log_perm log_bytes len input out_len out_bytes output v sq t entries read wrote entries' out_bytes'
+       ))
+
+[@@__reduce__]
+let verify_post_some_m_failure
+  (output: EXT.extern_ptr U8.t) // U.larray U8.t out_len)
+: Tot vprop
+= exists_ (fun s -> A.pts_to (EXT.gtake output) full_perm s)
+
+let verify_post_some_m
+  (tid:U16.t)
+  (log_perm:perm)
+  (log_bytes: AT.bytes)
+  (len: U32.t) // { len <> 0ul })
+  (input: EXT.extern_ptr U8.t) // U.larray U8.t len)
+  (out_len: U32.t)
+  (out_bytes: AT.bytes)
+  (output: EXT.extern_ptr U8.t) // U.larray U8.t out_len)
+  (v: option (v:V.verify_result { V.verify_result_complete len v }))
+  (sq: squash (check_verify_input tid len input out_len output))
+  (t: M.top_level_state)
+  (entries: _)
+: Tot vprop
+= match v with
+  | Some (V.Verify_success read wrote) ->
+    verify_post_some_m_success tid log_perm log_bytes len input out_len out_bytes output v sq t entries read wrote
+  | _ -> verify_post_some_m_failure output 
+
+[@@__reduce__]
+let verify_post_some
+  (tid:U16.t)
+  (log_perm:perm)
+  (log_bytes: AT.bytes)
+  (len: U32.t) // { len <> 0ul })
+  (input: EXT.extern_ptr U8.t) // U.larray U8.t len)
+  (out_len: U32.t)
+  (out_bytes: AT.bytes)
+  (output: EXT.extern_ptr U8.t) // U.larray U8.t out_len)
+  (v: option (v:V.verify_result { V.verify_result_complete len v }))
+  (sq: squash (check_verify_input tid len input out_len output))
+: Tot vprop
+= 
+    exists_ (fun t -> exists_ (fun entries ->
+      handle_pts_to t `star`
+      A.pts_to (EXT.gtake input) log_perm log_bytes `star`
+      verify_post_some_m tid log_perm log_bytes len input out_len out_bytes output v sq t entries
+    ))
+
+let verify_post
+  (tid:U16.t)
+  (log_perm:perm)
+  (log_bytes: AT.bytes)
+  (len: U32.t) // { len <> 0ul })
+  (input: EXT.extern_ptr U8.t) // U.larray U8.t len)
+  (out_len: U32.t)
+  (out_bytes: AT.bytes)
+  (output: EXT.extern_ptr U8.t) // U.larray U8.t out_len)
+  (res: verify_result len)
+: Tot vprop
+= match res with
+  | None -> verify_pre log_perm log_bytes input out_bytes output
+  | Some v ->
+    if check_verify_input tid len input out_len output
+    then verify_post_some tid log_perm log_bytes len input out_len out_bytes output v ()
+    else pure False
 
 val verify_log
-               (#t:Ghost.erased M.top_level_state)
-               (tid:_)
-               (#entries:Ghost.erased AEH.log)
+               (tid:U16.t)
                (#log_perm:perm)
                (#log_bytes:Ghost.erased AT.bytes)
-               (len: U32.t { len <> 0ul })
-               (input:U.larray U8.t len)
+               (len: U32.t)
+               (input: EXT.extern_ptr U8.t)
                (out_len: U32.t)
                (#out_bytes:Ghost.erased AT.bytes)
-               (output:U.larray U8.t out_len)
-  : STT (option (v:V.verify_result { V.verify_result_complete len v }))
-    (handle_pts_to t `star`
-     A.pts_to input log_perm log_bytes `star`
-     A.pts_to output full_perm out_bytes `star`
-     M.log_of_tid t tid entries)
-    (fun res ->
-       handle_pts_to t `star`
-       M.verify_post t tid entries log_perm log_bytes len input out_len out_bytes output res)
+               (output: EXT.extern_ptr U8.t)
+  : STT (verify_result len)
+    (verify_pre log_perm log_bytes input out_bytes output)
+    (fun res -> verify_post tid log_perm log_bytes len input out_len out_bytes output res)
+
+[@@__reduce__]
+let max_certified_epoch_post_some
+  (res: AEH.max_certified_epoch_result)
+: Tot vprop
+=
+  exists_ (fun t -> handle_pts_to t `star`
+    M.read_max_post t res)
+
+let max_certified_epoch_post
+  (res: option AEH.max_certified_epoch_result)
+: Tot vprop
+= match res with
+  | None -> emp
+  | Some res -> max_certified_epoch_post_some res
 
 val max_certified_epoch
-                        (#t:Ghost.erased M.top_level_state)
                         (_: unit)
-  : STT AEH.max_certified_epoch_result
-        (handle_pts_to t)
-        (fun res ->
-           handle_pts_to t `star`
-           M.read_max_post t res)
+  : STT (option AEH.max_certified_epoch_result)
+        emp
+        (fun res -> max_certified_epoch_post res)
